cryptis.v
@@ -1,7 +1,7 @@
 From mathcomp Require Import ssreflect.
 From stdpp Require Import gmap.
 From iris.algebra Require Import agree auth gset gmap list namespace_map.
-From iris.base_logic.lib Require Import auth saved_prop.
+From iris.base_logic.lib Require Import saved_prop.
 From iris.heap_lang Require Import notation proofmode.
 From cryptis Require Import lib term.
 
