primitives/comp.v
@@ -6,7 +6,7 @@ From mathcomp Require Import ssreflect.
 From mathcomp Require order.
 From stdpp Require Import gmap.
 From iris.algebra Require Import agree auth gset gmap namespace_map.
-From iris.base_logic.lib Require Import invariants auth.
+From iris.base_logic.lib Require Import invariants.
 From iris.heap_lang Require Import notation proofmode.
 From cryptis Require Import lib term.
 From cryptis.primitives Require Import notations.
