primitives/simple.v
@@ -2,7 +2,7 @@ From mathcomp Require Import ssreflect.
 From mathcomp Require order.
 From stdpp Require Import gmap.
 From iris.algebra Require Import agree auth gset gmap namespace_map.
-From iris.base_logic.lib Require Import invariants auth saved_prop.
+From iris.base_logic.lib Require Import invariants saved_prop.
 From iris.heap_lang Require Import notation proofmode.
 From iris.heap_lang.lib Require Import nondet_bool.
 From cryptis Require Import lib term cryptis.
